Cpc/TypePreservation/Base.lean
@@ -69,7 +69,7 @@ theorem typeof_value_model_eval_var
     __smtx_typeof_value (__smtx_model_eval M (SmtTerm.Var s T)) =
       __smtx_typeof (SmtTerm.Var s T) := by
   change __smtx_typeof_value (__smtx_model_lookup M s T) = T
-  exact hM s T hT
+  exact model_total_typed_lookup hM s T hT
 
 theorem typeof_value_model_eval_uconst
     (M : SmtModel)
@@ -80,7 +80,27 @@ theorem typeof_value_model_eval_uconst
     __smtx_typeof_value (__smtx_model_eval M (SmtTerm.UConst s T)) =
       __smtx_typeof (SmtTerm.UConst s T) := by
   change __smtx_typeof_value (__smtx_model_lookup M s T) = T
-  exact hM s T hT
+  exact model_total_typed_lookup hM s T hT
+
+theorem model_eval_var_of_uninhabited
+    (M : SmtModel)
+    (hM : model_total_typed M)
+    (s : smt_lit_String)
+    (T : SmtType)
+    (hT : ¬ type_inhabited T) :
+    __smtx_model_eval M (SmtTerm.Var s T) = SmtValue.NotValue := by
+  change __smtx_model_lookup M s T = SmtValue.NotValue
+  exact model_total_typed_lookup_uninhabited hM s T hT
+
+theorem model_eval_uconst_of_uninhabited
+    (M : SmtModel)
+    (hM : model_total_typed M)
+    (s : smt_lit_String)
+    (T : SmtType)
+    (hT : ¬ type_inhabited T) :
+    __smtx_model_eval M (SmtTerm.UConst s T) = SmtValue.NotValue := by
+  change __smtx_model_lookup M s T = SmtValue.NotValue
+  exact model_total_typed_lookup_uninhabited hM s T hT
 
 theorem typeof_value_model_eval_re_allchar
     (M : SmtModel) :
